\documentclass{article}
\usepackage[utf8]{inputenc}
\usepackage{fancyhdr}
\usepackage[margin=1.0in]{geometry}
\usepackage{amsmath}
\usepackage{changepage,stackrel}
\usepackage{graphicx}
\usepackage[inline]{enumitem}
\usepackage{enumitem}
\pagestyle{fancy}
\chead{Math 121 - Logarithmic, Exponential, and Inverse Trig Functions}
\begin{document}
\begin{enumerate}
\item Complete the following logarithmic and exponential rules
\begin{itemize}
    \item $x^ax^b=$?
    \item $(x^a)^b=$?
    \item $\frac{x^a}{x^b}$=?
    \item $\ln(ab) = $?
    \item $\ln{\frac{a}{b}}$=?
    \ite $\ln(x^a}$=?
\end{itemize}
    \item Assume that you have the functions $f(x)$ and $f^{-1}(x)$.
    \begin{itemize}
        \item What is $f(f^{-1}(x)) = $?
        \item Differentiate both sides of the equation above, then solve to get a formula for $[f^{-1}(x)]'$.
        \item In the formula above, use $f(x) = \ln(x)$ and $f^{-1}(x) = e^x$. What do you find?
        \item Similarly, what do you find if you use $f(x) = e^x$ and $f^{-1}(x) = \ln(x)$?
    \end{itemize}
    \item Now let $f(x) = \tan(x)$ and $f^{-1}(x) = \tan^{-1}(x)$.
    \begin{itemize}
        \item What is $f'(x)$?
        \item If $f^{-1}(x) = \tan^{-1}(x)$, what is $\tan(f^{-1}(x))$?
        \item What do we get if we plug in these values to the formula for $[f^{-1}]'$ from part 1?
        \item Use a trig identity (found in the back of the book if you aren't familiar with it), to get this formula in terms of tangents and inverse tangents. 
        \item Replace any instances of $\tan(f^{-1}(x))$ by $x$, and get the formula for the derivative of the inverse tangent function
    \end{itemize}
    \item Find $\frac{dy}{dx}$ if 
    \begin{itemize}
        \item $y = \ln(x)$
        \item $y = 5\ln(5x^3 + 4x -1$
        \item $y = \log_4(\sin(x))$
        \item $y = e^x$
        \item $y = e^{\tan(x)}$
        \item $y = 2^{x^2}$
        \item $y = \tan^{-1}(x)$
        \item $y = \tan^{-1}(\sin(x)$
    \end{itemize}
    \item Evaluate each of these integrals. Remember that a substitution might be needed.
    \begin{itemize}
        \item $\int \frac{1}{x} dx$
        \item $\int \frac{5}{x-1} dx$
        \item $\int \frac{6x^2 + 3}{2x^3 + 3x -1} dx$
        \item $\int 2x e^{x^2} dx$
        \item $\int \frac{1}{1 + x^2} dx$
        \item $\int \frac{\cos(x)}{1 + (\sin^2(x))} dx$
        \end{itemize}
\end{enumerate}
    
\end{enumerate}
\end{document}